feat(Compile_Nat) compile function calls
- We still need a function that resolves function symbols

Cook_Levin_IMP/IMP-_To_SAS+/Compile_Nat.thy
@@ -1,6 +1,25 @@
 theory Compile_Nat
-  imports IMP_Minus.Call_By_Prefixes
+  imports IMP_Minus.Call_By_Prefixes IMP_Minus.Big_Step_Small_Step_Equivalence
 begin
+
+fun measure_assoc where
+  "measure_assoc (Seq i1 i2) = Suc (measure_assoc i1 + measure_assoc i1 + measure_assoc i2)"
+| "measure_assoc (If _ i1 i2) = Suc (measure_assoc i1 + measure_assoc i2)"
+| "measure_assoc (While _ i) = Suc (measure_assoc i)"
+| "measure_assoc _ = 0"
+
+(* We could use this function instead of using ML but we should prove its correctness then *)
+function (sequential) assoc_right_Seq where
+  "assoc_right_Seq (Seq (Seq i1 i2) i3) = assoc_right_Seq (Seq i1 (Seq i2 i3))"
+| "assoc_right_Seq (Seq i1 i2) = Seq i1 (assoc_right_Seq i2)"
+| "assoc_right_Seq (If r i1 i2) = If r (assoc_right_Seq i1) (assoc_right_Seq i2)"
+| "assoc_right_Seq (While r i) = While r (assoc_right_Seq i)"
+| "assoc_right_Seq i = i"
+  by pat_completeness auto
+termination by (relation "measure measure_assoc") auto
+
+lemma big_step_t_Seq_assoc: "((c1 ;; c2) ;; c3, s) \<Rightarrow>\<^bsup>t\<^esup> s' \<longleftrightarrow> (c1 ;; (c2 ;; c3), s) \<Rightarrow>\<^bsup>t\<^esup> s'"
+  using compose_programs_1 by auto
 
 ML \<open>
   datatype tc_ast = If of (int * (tc_ast * tc_ast * tc_ast)) |
@@ -38,15 +57,11 @@ ML \<open>
           , [\<^Const>\<open>HOL.Not for \<open>\<^Const>\<open>HOL.eq \<^typ>\<open>nat\<close> for c \<open>\<^Const>\<open>Groups.zero \<^typ>\<open>nat\<close>\<close>\<close>\<close>\<close>\<close>, e1, e2]) =>
             If (~1, @{apply 3} build_tc_ast (c, e1, e2))
         (* Only allow condition of the form _ != 0 *)
-        | (\<^Const>\<open>HOL.If \<^typ>\<open>nat\<close>\<close>, _) => @{undefined}
+        | (\<^Const_>\<open>If\<close>, _) => @{undefined}
         | (f, args) => App (~1, (f, map build_tc_ast args))
     in
       t |> build_tc_ast |> index_tc_ast 0 |> snd
     end
-
-  fun reg_of_term idx (Const (s, _)) = (s, idx)
-    | reg_of_term idx (Free (s, _)) = (s, idx)
-    | reg_of_term idx (Var ((s, _), _)) = (s, idx)
 
   fun imp_of_tc_ast (App (index, (t, args))) =
     let
@@ -110,62 +125,6 @@ ML \<open>
       go (reg_var_of_indexname ret_reg) imp
     end
 
-  fun match_first a [] = raise Match
-    | match_first a (f :: fs) = case try f a of SOME b => b | NONE => match_first a fs
-
-  fun while_of_imp (f_name, f_typ) f_args (ret_reg, imp) =
-    let
-      fun string_of_indexname (n, i) = HOLogic.mk_string (n ^ "_" ^ Int.toString i)
-      fun mk_num n = \<^Const>\<open>N for \<open>HOLogic.mk_number \<^typ>\<open>nat\<close> n\<close>\<close>
-      fun mk_var n = \<^Const>\<open>V for n\<close>
-      val mk_local_var = mk_var o string_of_indexname
-      fun mk_atom a = \<^Const>\<open>A for a\<close>
-      
-      val cont_reg = HOLogic.mk_string "continue"
-      fun mk_continue n = \<^Const>\<open>Assign for cont_reg \<open>mk_atom (mk_num n)\<close>\<close>
-
-      fun while_of_call f args = @{undefined}
-      fun while_of_tailcall args = @{undefined}
-
-      fun go Skip = \<^Const>\<open>SKIP\<close>
-        | go (Seq (imp1, imp2)) = \<^Const>\<open>Seq for \<open>go imp1\<close> \<open>go imp2\<close>\<close>
-        | go (Copy (reg1, reg2)) =
-            \<^Const>\<open>Assign for \<open>string_of_indexname reg1\<close> \<open>mk_atom (mk_local_var reg2)\<close>\<close>
-        | go (IfNeqZero (_, (reg, imp1, imp2))) =
-            \<^Const>\<open>If for \<open>string_of_indexname reg\<close> \<open>go imp1\<close> \<open>go imp2\<close>\<close>
-        | go (Assign (reg, (g, args))) =
-            let
-              val nocall_cases =
-                [ mk_atom o mk_num o snd o HOLogic.dest_number
-                , (fn \<^Const>\<open>Groups.plus \<^typ>\<open>nat\<close>\<close> =>
-                    case args of [arg1, arg2] => \<^Const>\<open>Plus for \<open>mk_local_var arg1\<close> \<open>mk_local_var arg2\<close>\<close>)
-                , (fn \<^Const>\<open>Groups.minus \<^typ>\<open>nat\<close>\<close> =>
-                    case args of [arg1, arg2] => \<^Const>\<open>Sub for \<open>mk_local_var arg1\<close> \<open>mk_local_var arg2\<close>\<close>)
-                , (fn (Var ((n, _), _)) => Long_Name.base_name f_name ^ "_" ^ n
-                                           |> HOLogic.mk_string |> mk_var |> mk_atom)
-                ]
-              fun mk_assign rhs = \<^Const>\<open>Assign for \<open>string_of_indexname reg\<close> rhs\<close>
-
-              fun mk_tailcall () =
-                let
-                  fun mk_assign_arg (f_arg, arg) =
-                    \<^Const>\<open>Assign for \<open>HOLogic.mk_string f_arg\<close> \<open>string_of_indexname arg\<close>\<close>
-                  val mk_assign_args = 
-                    map mk_assign_arg (f_args ~~ args)
-                    |> (fn ass => fold (fn e1 => fn e2 => \<^Const>\<open>Seq for e1 e2\<close>) ass \<^Const>\<open>SKIP\<close>)
-                in
-                  \<^Const>\<open>Seq for mk_assign_args \<open>mk_continue 1\<close>\<close>
-                end
-              val call_cases =  
-                [ (fn Const (f_name, f_typ) => mk_tailcall ())
-                ]
-            in
-              match_first g
-                (map (curry (op o) mk_assign) nocall_cases @ call_cases)
-            end
-    in
-      \<^Const>\<open>Seq for \<open>mk_continue 1\<close> \<^Const>\<open>While for cont_reg \<^Const>\<open>Seq for \<open>mk_continue 0\<close> \<open>go imp\<close>\<close>\<close>\<close>
-    end
 
   fun define_let_of_def def binding lthy =
     let
@@ -177,7 +136,6 @@ ML \<open>
            def_body
         |> curry Term.subst_bounds (args_vars |> rev)
         |> tc_ast_of_term
-        |> @{print}
         |> imp_of_tc_ast
         |> let_of_imp
         |> fold_rev lambda args_vars
@@ -185,24 +143,121 @@ ML \<open>
       Local_Theory.define ((binding, NoSyn), ((Thm.def_binding binding, []), let_def)) lthy
       |> snd
     end
+
+  fun match_first a [] = raise TERM ("No match", [a])
+    | match_first a (f :: fs) = case try f a of SOME b => b | NONE => match_first a fs
+
+  fun IMP_Minus_of_imp f (f_ret_name, f_arg_names) lookup_fn (ret_reg, imp) =
+    let
+      fun string_of_indexname (n, i) = HOLogic.mk_string (n ^ "_" ^ Int.toString i)
+      fun mk_local_V n = \<^Const>\<open>V for \<open>string_of_indexname n\<close>\<close>
+  
+      fun mk_N n = \<^Const>\<open>N for \<open>HOLogic.mk_number \<^typ>\<open>nat\<close> n\<close>\<close>
+  
+      val cont_reg = HOLogic.mk_string "continue"
+      fun mk_continue n = \<^Const>\<open>Assign for cont_reg \<^Const>\<open>A for \<open>mk_N n\<close>\<close>\<close>
+      fun mk_While p =
+        \<^Const>\<open>Seq for \<open>mk_continue 1\<close>
+                      \<^Const>\<open>While for cont_reg \<^Const>\<open>Seq for \<open>mk_continue 0\<close> p\<close>\<close>\<close>
+  
+      fun mk_bop bop [arg1, arg2] = bop $ mk_local_V arg1 $ mk_local_V arg2
+
+      fun mk_Seq es = fold_rev (fn e1 => fn e2 => \<^Const>\<open>Seq for e1 e2\<close>) es \<^Const>\<open>SKIP\<close>
+
+      fun mk_assign_arg (arg_name, arg) =
+        \<^Const>\<open>Assign for arg_name \<^Const>\<open>A for \<open>mk_local_V arg\<close>\<close>\<close>
+
+      fun mk_tailcall args =
+        map mk_assign_arg (map HOLogic.mk_string f_arg_names ~~ args) @ [mk_continue 1]
+        |> mk_Seq
+
+      fun mk_fun_arg prefix arg_name =
+        \<^Const>\<open>List.append \<^typ>\<open>char list\<close> for \<open>HOLogic.mk_string prefix\<close> \<open>HOLogic.mk_string arg_name\<close>\<close>
+
+      fun mk_call reg g args (prefix, (ret_name, args_names)) =
+        map mk_assign_arg (map (mk_fun_arg prefix) args_names ~~ args) @
+        [ \<^Const>\<open>com_add_prefix for \<open>HOLogic.mk_string prefix\<close> \<open>Const g\<close>\<close>
+        , \<^Const>\<open>Assign for reg \<^Const>\<open>A for \<^Const>\<open>V for \<open>HOLogic.mk_string ret_name\<close>\<close>\<close>\<close>
+        ]
+        |> mk_Seq
+        
+
+      fun go Skip = \<^Const>\<open>SKIP\<close>
+        | go (Seq (imp1, imp2)) = \<^Const>\<open>Seq for \<open>go imp1\<close> \<open>go imp2\<close>\<close>
+        | go (Copy (reg1, reg2)) =
+            \<^Const>\<open>Assign for \<open>string_of_indexname reg1\<close> \<^Const>\<open>A for \<open>mk_local_V reg2\<close>\<close>\<close>
+        | go (IfNeqZero (_, (reg, imp1, imp2))) =
+            \<^Const>\<open>If for \<open>string_of_indexname reg\<close> \<open>go imp1\<close> \<open>go imp2\<close>\<close>
+        | go (Assign (reg, (g, args))) =
+            let
+              val base_cases_rhs =
+                [ (fn n => \<^Const>\<open>A for \<open>n |> HOLogic.dest_number |> snd |> mk_N\<close>\<close>)
+                , (fn \<^Const>\<open>Groups.plus \<^typ>\<open>nat\<close>\<close> => mk_bop \<^Const>\<open>Plus\<close> args)
+                , (fn \<^Const>\<open>Groups.minus \<^typ>\<open>nat\<close>\<close> => mk_bop \<^Const>\<open>Sub\<close> args)
+                , (fn (Var ((n, _), _)) =>
+                    \<^Const>\<open>A for \<^Const>\<open>V for \<open>HOLogic.mk_string n\<close>\<close>\<close>)
+                ]
+              fun mk_assign rhs = \<^Const>\<open>Assign for \<open>string_of_indexname reg\<close> rhs\<close>
+              val base_cases = map (curry (op o) mk_assign) base_cases_rhs
+
+              val call_cases =  
+                [ (fn Const f' => if f' = f then mk_tailcall args else raise Match)
+                , (fn Const f' => mk_call (string_of_indexname reg) f' args (lookup_fn f'))
+                ]
+            in
+              match_first g (base_cases @ call_cases)
+            end
+    in
+      \<^Const>\<open>Seq for \<open>go imp |> mk_While\<close>
+                    \<^Const>\<open>Assign for \<open>HOLogic.mk_string f_ret_name\<close> \<^Const>\<open>A for \<open>mk_local_V ret_reg\<close>\<close>\<close>\<close>
+    end
+
+  fun rm_SKIP \<^Const>\<open>Seq for \<^Const>\<open>SKIP\<close> e2\<close> = rm_SKIP e2
+    | rm_SKIP \<^Const>\<open>Seq for e1 \<^Const>\<open>SKIP\<close>\<close> = rm_SKIP e1
+    | rm_SKIP \<^Const>\<open>Seq for e1 e2\<close> = \<^Const>\<open>Seq for \<open>rm_SKIP e1\<close> \<open>rm_SKIP e2\<close>\<close>
+    | rm_SKIP \<^Const>\<open>If for r e1 e2\<close> = \<^Const>\<open>If for r \<open>rm_SKIP e1\<close> \<open>rm_SKIP e2\<close>\<close>
+    | rm_SKIP \<^Const>\<open>While for r e\<close> = \<^Const>\<open>While for r \<open>rm_SKIP e\<close>\<close>
+    | rm_SKIP t = t
+
+  fun assoc_right_Seq \<^Const>\<open>Seq for \<^Const>\<open>Seq for e1 e2\<close> e3\<close> =
+        assoc_right_Seq \<^Const>\<open>Seq for e1 \<^Const>\<open>Seq for e2 e3\<close>\<close>
+    | assoc_right_Seq \<^Const>\<open>Seq for e1 e2\<close> = \<^Const>\<open>Seq for e1 \<open>assoc_right_Seq e2\<close>\<close>
+    | assoc_right_Seq \<^Const>\<open>If for r e1 e2\<close> =
+        \<^Const>\<open>If for r \<open>assoc_right_Seq e1\<close> \<open>assoc_right_Seq e2\<close>\<close>
+    | assoc_right_Seq \<^Const>\<open>While for r e\<close> = \<^Const>\<open>While for r \<open>assoc_right_Seq e\<close>\<close>
+    | assoc_right_Seq e = e
+  
 \<close>
+
+ML \<open>Library.foldr\<close>
 
 definition "test (x :: nat) \<equiv> \<lambda>y. if x + y \<noteq> 0 then if y \<noteq> 0 then y else x else 0"
 
+fun test1 :: "nat \<Rightarrow> nat \<Rightarrow> nat" where
+  "test1 x y = (if x \<noteq> 0 then test1 (x - 1 - 1) (y + 1) else y)"
+
+declare [[ML_print_depth=500]]
 ML \<open>
     let
+      val f_def = @{thm eq_reflection[OF test1.simps(1)]}
       val (args, def_body) =
-        Local_Defs.abs_def_rule @{context} @{thm test_def}
+        Local_Defs.abs_def_rule @{context} f_def
         |> Thm.rhs_of |> Thm.term_of |> Term.strip_abs
-      val args_vars = map (Var o @{apply 2 (1)} (fn s => (s, 0))) args
+
+      val (f_name, f_typ) = f_def |> Thm.lhs_of |> Thm.term_of |> Term.head_of |> Term.dest_Const
+      val f_ret_name = Long_Name.base_name f_name ^ "_ret"
+      fun mk_arg_name arg_name = Long_Name.base_name f_name ^ "_" ^ arg_name
+      val f_args = map (@{apply 2 (1)} mk_arg_name) args
+      val f_arg_vars = map (Var o @{apply 2 (1)} (fn n => (n, 0))) f_args
     in
            def_body
-        |> curry Term.subst_bounds (args_vars |> rev)
+        |> curry Term.subst_bounds (f_arg_vars |> rev)
         |> tc_ast_of_term
-        |> @{print}
         |> imp_of_tc_ast
         |> @{print}
-        |> while_of_imp (\<^Const>\<open>test\<close> |> Term.dest_Const) (map fst args)
+        |> IMP_Minus_of_imp (f_name, f_typ) (f_ret_name, map fst f_args) (fn _ => @{undefined})
+        |> rm_SKIP
+        |> assoc_right_Seq
         |> Thm.cterm_of @{context}
     end
 \<close>
